Java/src/Java/Logic/SpecLogic.v
@@ -1,4 +1,4 @@
-Require Import Later Lang Program ILogic ILEmbed ILInsts Maps.
+Require Import Later Lang Program ILogic ILEmbed ILInsts Containers.Maps.
 
 Local Existing Instance ILLaterNat.
 Local Existing Instance ILLaterNatOps.
