Java/src/Java/Semantics/SemCmd.v
@@ -1,0 +1,387 @@
+Require Import SepAlg OpenILogic Charge.SepAlg.SepAlgMap. 
+Require Import MapInterface MapFacts.
+Require Import ILInsts ILogic ILEmbed Open Subst Stack.
+Require Import Program Java.Logic.SpecLogic Heap ProtocolLogic Lang Traces Java.Logic.ST.
+Require Import AssertionLogic ST Util.
+
+Import SepAlgNotations.
+
+Set Implicit Arguments.
+Unset Strict Implicit.
+Set Maximal Implicit Insertion.
+
+Section Compatability.
+
+  Program Fixpoint Comp (Pr : Prog_wf) (n : nat) (pr : STs) (tr : trace) (Q : psasn) : Prop :=
+    match tr with 
+      | t_end => False
+      | t_fail => False
+      | t_send x v h tr' => match (find x pr) with
+          | Some (st_send z P T) =>  P (stack_add z v (stack_empty _)) Pr n h /\ Comp Pr (n - 1) (add x (subst_ST z v T) pr) tr' Q
+          | _ => False
+        end
+      | t_recv x tr' => match (find x pr) with
+          | Some (st_recv z P T) =>  forall v h, P (stack_add z (vptr v) (stack_empty _)) Pr n h ->
+                                                 Comp Pr (n - 1) (add x (subst_ST z v T) pr) (tr' v h) Q
+          | _ => False
+        end
+      | t_start x tr' tr'' => exists (T : ST), 
+          Comp Pr (n-1) (add x T (empty _)) tr' 
+               (fun s => mk_pasn (fun pr' Pr n _ => (forall c', In c' pr' -> MapsTo c' st_end pr') /\ 
+          			                               forall m, m <= n -> forall Pr', Prog_wf_sub Pr Pr' ->
+          			                                  Comp Pr' m (add x (dual T) pr) tr'' Q) _ _ _ _)
+      | t_tau s h _ tr' => match tr' with
+                         | t_end => Q s pr Pr n h 
+                         | _     => Comp Pr (n - 1) pr tr' Q
+                         end
+    end.
+    Next Obligation.
+	  split; [|assumption].
+	  intros. rewrite <- H. apply H0.
+	  rewrite H. assumption.
+	Defined.
+    Next Obligation.
+	  split. assumption. intros. eapply H1.
+	  assumption. transitivity P'; assumption.
+	Defined.
+
+  Local Transparent ILPre_Ops.
+  Local Transparent ILFun_Ops.
+
+  Lemma Comp_entails Pr pr tr n (Q Q' : psasn) (HQQ' : Q |-- Q') (H : Comp Pr n pr tr Q) : 
+  	Comp Pr n pr tr Q'.
+  Proof with eauto.
+    intros.
+    generalize dependent pr. generalize dependent n. generalize dependent Pr. generalize dependent Q. generalize dependent Q'.
+    induction tr; intros; simpl in *...
+    - remember (find s pr); destruct o...
+      destruct s0; try assumption; destruct H...  
+    - remember (find s pr); destruct o...
+      destruct s0; try assumption... 
+    - destruct H as [T ?]; exists T.
+      eapply IHtr1; [| apply H].
+      intros. simpl in *. destruct H0; split; [assumption|].
+      intros; eapply IHtr2. eapply HQQ'. apply H1. assumption. assumption.
+    - destruct tr; try eapply HQQ'; try eassumption; try eapply IHtr; eassumption.
+  Qed.
+(*
+  Lemma Comp_split : forall Pr n pr tr (P Q : nat -> STs -> Prop), Comp Pr n pr tr P -> Comp Pr n pr tr Q -> Comp Pr n pr tr (fun n pr' => P n pr' /\ Q n pr').
+  Proof with auto.
+    intros.
+    generalize dependent pr. generalize dependent n.
+    induction tr; intros; simpl in *... 
+    - remember (find s pr); destruct o...
+      destruct s0; try assumption; destruct H, H0...
+    - remember (find s pr); destruct o...
+      destruct s0; try assumption...
+    - (* create a witness that is the pointwise conjugation of T from H and T0 from H0 Ø)
+       * So !z,P.T' + !z.P0.T0' becomes !z.{P /\ P0}.tail(T', T0') *)
+      admit (* fangel, this needs a solution! *).
+  Qed.
+
+  Lemma Comp_partial : forall Pr n m k pr tr tr' (P Q : nat -> STs -> Prop), 
+     n = trace_length tr ->
+     n + m  <= k -> 
+     Comp Pr k pr tr P -> 
+     (forall pr, P m pr -> Comp Pr m pr tr' Q) -> 
+     Comp Pr k pr (trace_append tr tr') Q.
+  Proof with auto.
+    admit.
+Admitted.
+  (*
+    intros.
+    generalize dependent pr. generalize dependent n.
+    induction tr; intros; simpl in *; [subst | ..]...
+    - remember (find s pr); destruct o...
+      destruct s0; try assumption; destruct H0; split; [solve_model H0 |]. 
+      assert (n - 1 = trace_length tr) by omega.
+      specialize (IHtr _ H3); replace (n - 1 + m) with (n + m - 1) in * by omega...
+    - remember (find s pr); destruct o...
+      destruct s0; try assumption; intro.
+      assert (n - 1 = trace_length tr) by omega. 
+      specialize (IHtr _ H3); replace (n - 1 + m) with (n + m - 1) in * by omega...
+    - destruct H0 as [T ?]; exists T. 
+      eapply Comp_entails; [| apply H0].
+      intros. simpl in H2; destruct H2.
+      split; [assumption |].
+      
+      assert (m0 = trace_length tr2) by admit (* fangel, test *). 
+      eapply IHtr2.
+      specialize (IHtr2 _ H4); replace (n - 1 + m) with (n + m - 1) in * by omega..
+    - assert (n - 1 = trace_length tr) by omega.
+      specialize (IHtr _ H2); replace (n - 1 + m) with (n + m - 1) in * by omega...
+  Qed. *)
+*)
+End Compatability.
+
+Section Commands.
+
+  Definition semCmdType := Prog_wf -> stack -> heap -> NS.t -> trace -> Type.
+  Definition safe (c : semCmdType) Pr s h cl := forall tr, c Pr s h cl tr -> trace_safe tr.
+
+  Inductive frame_trace (frame : heap) : trace -> trace -> Type :=
+  	| ft_end : frame_trace frame t_end t_end
+  	| ft_fail tr : frame_trace frame t_fail tr
+  	| ft_tau tr tr' s big cl h : frame_trace frame tr tr' ->
+  	                 sa_mul h frame big -> frame_trace frame (t_tau s h cl tr) (t_tau s big cl tr')
+  	| ft_send tr tr' x v h big : frame_trace frame tr tr' ->
+  	                            sa_mul h frame big -> frame_trace frame (t_send x v h tr) (t_send x v big tr')
+  	| ft_recv f g c : (forall x h, frame_trace frame (f x h) (g x h)) -> frame_trace frame (t_recv c f) (t_recv c g)
+  	| ft_start c tr tr' tr'' : frame_trace frame tr tr' -> frame_trace frame (t_start c tr'' tr) (t_start c tr'' tr').
+
+  Definition frame_property (c : semCmdType) : Type :=
+    forall Pr s (big frame h : heap) cl tr
+      (HFrame : @sa_mul heap HeapSepAlgOps h frame big) 
+      (HSem   : c Pr s big cl tr),
+      sigT (fun tr' => (frame_trace frame tr' tr * c Pr s h cl tr')%type).
+(*
+  Definition frame_property (c : semCmdType) :=
+    forall Pr s s' (big big' frame h : heap) cl cl' tr
+      (HFrame : @sa_mul heap HeapSepAlgOps h frame big) 
+      (HSafe  : safe c Pr m s h cl tr)
+      (HSem   : c Pr s big cl tr(* (Some (s', (big', cl'))))*),
+      exists h', sa_mul h' frame big' /\ c Pr n s h cl tr (Some (s', (h', cl'))).
+*)
+  Record semCmd := {
+    cmd_rel   :> Prog_wf -> stack -> heap -> NS.t -> trace -> Prop;
+    cmd_zero  :  forall Pr s h cl, ~(cmd_rel Pr s h cl t_end);
+    cmd_frame : frame_property cmd_rel
+  }.
+  Print semCmd.
+(*
+  Definition not_modifies (c : semCmdType) x : Prop :=
+    forall Pr s s' h h' cl cl' n tr (HSem : c Pr n s h cl tr (Some (s', (h', cl')))),
+      s x = s' x.
+
+  Lemma safe_zero : forall (c : semCmd) Pr s h cl tr, safe c Pr 0 s h cl tr.
+  Proof.
+    unfold safe; intros; apply cmd_zero.
+  Qed.
+  
+  Global Opaque sa_mul.
+
+  Implicit Arguments Build_semCmd [].
+
+  Program Definition later_cmd (c : semCmd) : semCmd := Build_semCmd
+    (fun Pr n => match n return stack -> heap -> NS.t -> trace -> option (stack * (heap * NS.t) ) -> Prop with
+                  | O => fun _ _ _ _ _ => False
+                  | S n => c Pr n end) _ _.
+  Next Obligation.
+    unfold frame_property; intros.
+    destruct n as [| n]; unfold safe in HSafe; simpl in *; [contradiction |].
+    eapply cmd_frame; eauto. 
+    intros m HLe HFail; apply (HSafe (S m)); auto with arith.
+  Qed.
+*)
+
+  Inductive skip_sem : semCmdType :=
+  | s_ok : forall Pr s h cl, skip_sem Pr s h cl (t_tau s h cl t_end).
+  Program Definition skip_cmd := @Build_semCmd skip_sem _ _.
+  Next Obligation.
+    intros H. inversion H.
+  Qed.
+  Next Obligation.
+	unfold frame_property.
+	intros. inversion HSem; subst.
+	admit.
+  Qed.
+
+  (* Seq *)
+
+  Inductive trace_append_cmd (Pr : Prog_wf) (c : semCmd) : trace -> trace -> Type :=
+    | ta_fail : trace_append_cmd Pr c t_fail t_fail
+  	| ta_send p v h tr tr' : trace_append_cmd Pr c tr tr' ->
+  	                         trace_append_cmd Pr c (t_send p v h tr) (t_send p v h tr')
+  	| ta_recv p f g: (forall v h, trace_append_cmd Pr c (f v h) (g v h)) ->
+  	                              trace_append_cmd Pr c (t_recv p f) (t_recv p g)
+  	| ta_bc s h tr cl : c Pr s h cl tr -> trace_append_cmd Pr c (t_tau s h cl t_end) (t_tau s h cl tr)
+  	| ta_tau s h tr tr' cl : trace_append_cmd Pr c tr tr' -> 
+  	                         trace_append_cmd Pr c (t_tau s h cl tr) (t_tau s h cl tr').
+  
+    Lemma trace_append_cmd_frame_trace Pr c tr tr' tr'' frame
+    	(Hc : trace_append_cmd Pr c tr tr') (HFrame : frame_trace frame tr'' tr) :
+    	sigT (fun tr''' => (trace_append_cmd Pr c tr'' tr''' * frame_trace frame tr''' tr')%type).
+    Proof with eauto.
+      generalize dependent tr'. induction HFrame; intros.
+      + inversion Hc.
+      + exists t_fail; try repeat constructor.
+      + inversion Hc; subst.
+        inversion HFrame; subst.
+        edestruct (@cmd_frame c) as [tr2 [HFrame2 HSem2]]...
+        exists (t_tau s h cl tr2).
+        split.
+        constructor; assumption.
+        constructor; assumption.
+        exists (t_tau s h cl t_fail). split; try repeat constructor. assumption.
+        specialize (IHHFrame _ X).
+        destruct IHHFrame as [tr''' [H1 H2]].
+        exists (t_tau s h cl tr'''). 
+        split; constructor; assumption.
+      + inversion Hc; subst.
+        specialize (IHHFrame _ X).
+        destruct IHHFrame as [tr''' [H1 H2]].
+        exists (t_send x v h tr''').
+        split; constructor; assumption.
+      + inversion Hc; subst.
+        exists (t_recv c0 (fun x h => match X x h (g0 x h) (X0 x h) with existT w P => w end)).
+	    split; constructor; intros.
+	    - destruct (X v h (g0 v h) (X0 v h)) as [tr2 [H _]]; apply H.
+	    - destruct (X x h (g0 x h) (X0 x h)) as [tr2 [_ H]]; apply H.
+      + inversion Hc.
+   Qed.
+
+
+    Inductive seq_sem (c1 c2 : semCmd) : semCmdType :=
+    | seq_ok : forall Pr s h cl tr tr',
+    	c1 Pr s h cl tr ->
+    	trace_append_cmd Pr c2 tr tr' ->
+    	seq_sem c1 c2 Pr s h cl tr'.
+  Program Definition seq_cmd c1 c2 := @Build_semCmd (seq_sem c1 c2) _ _.
+  Next Obligation.
+	intros H; inversion H; subst. inversion X.
+  Qed.
+  Next Obligation with eauto using seq_sem.
+    unfold frame_property; intros.
+    inversion HSem; subst.
+    edestruct (@cmd_frame c1) as [tr1 [HFrame1 Hsem1]]...
+            
+    pose proof (trace_append_cmd_frame_trace X HFrame1).
+    destruct X0 as [tr' [H1 H2]].
+    exists tr'. split; [assumption|].
+    eapply seq_ok; eassumption.
+  Qed.
+
+  (* Nondet *)
+  Inductive nondet_sem (c1 c2 : semCmd) : semCmdType :=
+  | nondetL   : forall Pr s h cl tr,
+      c1 Pr s h cl tr ->
+      (nondet_sem c1 c2) Pr s h cl tr
+   | nondetR   : forall Pr s h tr cl,
+      c2 Pr s h cl tr ->
+      nondet_sem c1 c2 Pr s h cl tr.
+  Program Definition nondet_cmd c1 c2 := @Build_semCmd (nondet_sem c1 c2) _ _.
+  Next Obligation.
+    intros H; inversion H; subst;
+    apply cmd_zero in H0; assumption.
+  Qed.
+  Next Obligation with eauto using nondet_sem.
+	intros Pr s big frame h cl tr HFrame HSem.
+	inversion HSem; subst.
+	+ edestruct (@cmd_frame c1)...
+	  exists x. destruct p as [H1 H2]. split; [assumption|].
+	  apply nondetL; assumption.
+	+ edestruct (@cmd_frame c2)...
+	  exists x; destruct p as [H1 H2]; split; [assumption|].
+	  apply nondetR; assumption.
+  Qed.
+
+  (* Kleene star *)
+
+  Inductive kleene_sem (c : semCmd) : semCmdType :=
+  | kleene_emp       : forall Pr s h cl,
+      kleene_sem c Pr s h cl (t_tau s h cl t_end)
+  | kleene_step_ok   : forall Pr s h tr tr1 cl,
+      c Pr s h cl tr ->
+      trace_append_cmd Pr c tr tr1 ->
+      kleene_sem c Pr s h cl tr1.
+  Program Definition kleene_cmd c := @Build_semCmd (kleene_sem c) _ _.
+  Next Obligation.
+	intros H; inversion H; subst. inversion X. 
+  Qed.
+  Next Obligation with eauto using kleene_sem.
+    unfold frame_property; intros.
+    generalize dependent h. induction HSem; intros.
+    + exists (t_tau s h0 cl t_end).
+      split; try repeat constructor; assumption.
+    + edestruct (@cmd_frame c) as [tr2 [HFrame1 Hsem1]]...            
+      pose proof (trace_append_cmd_frame_trace t HFrame1).
+      destruct X as [tr' [H1 H2]].
+      exists tr'. split; [assumption|].
+      eapply kleene_step_ok; eassumption.
+  Qed.
+
+  (* TODO: update the description
+     assume command -- this command is a bit of a hack that just skips if
+     a check holds and loops otherwise, this way allowing to encode if/while
+     using nondeterministic choice/Kleene star *)
+  Inductive assume_sem (p : vlogic) : semCmdType :=
+  | assume_ok : forall Pr s h cl, p s -> assume_sem p Pr s h cl (t_tau s h cl t_end).
+  Program Definition assume_cmd P := @Build_semCmd (assume_sem P) _ _.
+  Next Obligation.
+    intros H; inversion H.
+  Qed.
+  Next Obligation.
+    unfold frame_property; intros.
+    induction HSem.
+    exists (t_tau s h cl t_end).
+    split; try repeat constructor; assumption.
+  Qed.
+
+(*
+  Lemma assume_inv Pr e n s s0 h h0 cl cl0 tr (HSem : assume_cmd e Pr n s h cl tr (Some (s0, (h0, cl0)))) : 
+      s = s0 /\ h = h0.
+  Proof.  
+    intros; remember (Some (s0, (h0, cl0))); induction HSem; subst;
+    try inversion Heqo; intuition.
+  Qed.
+*)
+  Inductive assert_sem (p : vlogic) : semCmdType :=
+  | assert_ok   : forall Pr s h cl (HP : p s),
+    assert_sem p Pr s h cl (t_tau s h cl t_end)
+  | assert_fail : forall Pr s h cl (HNP : ~p s),
+    assert_sem p Pr s h cl t_fail.
+  Program Definition assert_cmd p := @Build_semCmd (assert_sem p) _ _.
+  Next Obligation.
+    intros H; inversion H.
+  Qed.
+  Next Obligation with eauto using assert_sem.
+    unfold frame_property; intros.
+    inversion HSem; subst...
+    + exists (t_tau s h cl t_end); split; try repeat constructor; assumption.
+    + exists t_fail; split; try repeat constructor; assumption.
+  Qed.
+
+  (* |= {p}c{q} *)
+  Program Definition sem_triple (p q : psasn) (c : semCmd) : spec :=
+    mk_spec (fun P n => forall P' m s h cl STs, Prog_wf_sub P P' -> m <= n -> 
+                                           p s STs P' m h ->
+       (forall tr, c P' s h cl tr -> Comp P' m STs tr q)
+      		
+      
+    ) _ _.
+  Next Obligation.
+	eapply H; try eassumption; omega.
+  Qed.
+  Next Obligation.
+	eapply H0; try eassumption. transitivity P'; assumption.
+  Qed.
+End Commands.
+
+
+  Local Transparent ILPre_Ops.
+  Local Transparent ILFun_Ops.
+  
+  Add Parametric Morphism : sem_triple with signature
+    lentails --> lentails ++> eq ==> lentails
+    as sem_triple_entails_m.
+  Proof. 
+	intros p p' Hp q q' Hq c n x H P m s h cl pr HP Hmn Hp' tr HSem.
+	apply Hp in Hp'. 
+	specialize (H _ _ _ _ cl pr HP Hmn Hp' tr HSem).
+	eapply Comp_entails; eassumption.
+  Qed.
+
+  Add Parametric Morphism : sem_triple with signature
+    lequiv ==> lequiv ==> eq ==> lequiv
+    as sem_triple_lequiv_m.
+  Proof. 
+    split.
+    + rewrite H, H0; reflexivity.
+    + rewrite <- H, <- H0; reflexivity.
+  Qed.
+
+
+Implicit Arguments Build_semCmd [].
+
+Notation "{{ p }} c {{ q }}" := (sem_triple p q c) (at level 89,
+  format "{{ p }} '/ '  c '/ '  {{ q }}").
