Java/src/Java/Semantics/SemCmdRules.v
@@ -1,0 +1,289 @@
+Require Import SemCmd ILogic BILogic ILInsts BILInsts.
+Require Import OpenILogic Later ProtocolLogic AssertionLogic SpecLogic ILEmbed Open.
+Require Import Stack Subst Lang Util Lists.List.
+Require Import FunctionalExtensionality ST Traces.
+Require Import ExtLib.Tactics.
+
+Set Implicit Arguments.
+Unset Strict Implicit.
+Set Maximal Implicit Insertion.
+
+Open Scope open_scope.
+
+	Local Transparent ILPre_Ops.
+    Local Transparent ILFun_Ops.
+	Local Transparent BILPre_Ops.
+    Local Transparent BILFun_Ops.
+    Local Transparent ILLaterPreOps.
+    Local Transparent ILLaterNatOps.
+    Local Transparent EmbedPSasnSasnOp.
+    Local Transparent EmbedILFunDropOp.
+    Local Transparent EmbedILFunOp.
+    
+    
+    Ltac opt_destruct :=
+        match goal with
+          | H : context [match ?trm with | Some _ => _ | None => _ end] |- _ => 
+            let o := fresh "o" in remember trm as o; destruct o
+        end.
+
+
+Section Rules.
+
+  Section StructuralRules.
+
+    Lemma rule_of_consequence (P P' Q Q' : psasn) (c : semCmd)
+      (HPre  : P  |-- P')
+      (HPost : Q' |-- Q ) :
+      {{P'}}c{{Q'}} |-- {{P}}c{{Q}}.
+    Proof.
+      intros n Pr Hc Pr' m s h cl pr HPr Hmn HP; simpl.
+      specialize (Hc _ _ s h cl pr HPr Hmn).
+      + intros.
+       eapply Comp_entails; [intros; apply HPost; apply H0 |].
+       apply Hc; try assumption.
+       apply HPre; assumption.
+    Qed.
+
+
+
+	Local Existing Instance EmbedPSasnSasnOp.
+
+	Fixpoint trace_not_modifies (s : stack) (x : var) (tr : trace) :=
+        match tr with
+          | t_end => False
+          | t_fail => True
+          | t_tau s' _ _ tr => 
+          	match tr with 
+          	  | t_end => s x = s' x
+          	  | _ => trace_not_modifies s x tr
+            end
+          | t_send c v h tr => trace_not_modifies s x tr
+          | t_recv c f => forall v h, trace_not_modifies s x (f v h)
+          | t_start c tr tr' => trace_not_modifies s x tr'
+        end.
+		
+(*
+    Definition not_modifies (c : semCmd) (x : var) : Prop :=
+      forall PP s h cl tr , trace_not_modifies s x tr.
+
+*)
+    
+ 
+    Lemma frame_rule : forall (P Q R : psasn) (c : semCmd) (xs: list var)
+      (HMod : forall PP s h cl tr (HSem : c PP s h cl tr) x, ~ In x xs -> trace_not_modifies s x tr),
+      {{ P }} c {{ Q }} |--
+      {{ P ** R }} c {{ Q ** Exists vs, apply_subst R (subst_fresh vs xs) }}.
+    Proof with eauto.
+      intros.
+      intros P' n HSem P'' m s big cl STs HP'P'' Hmn HPR tr Hc. 
+      destruct HPR as [pr [prframe [HPRFrame [h [frame [HFrame [HP HR]]]]]]].
+      edestruct (@cmd_frame c)... destruct p as [H1 H2].
+      specialize (HSem P'' m s h cl pr HP'P'' Hmn HP _ H2).
+      specialize (HMod P'' s big cl tr Hc).
+      clear -HSem HR H1 HPRFrame HFrame HMod.
+      generalize dependent m; generalize dependent STs. generalize dependent pr. induction H1; intros.
+      + inversion HSem.
+      + inversion HSem.
+      + simpl in HSem. destruct tr.
+        - inversion H1; subst.
+          exists pr, prframe, HPRFrame, h0, frame, s1.
+          split; [apply HSem|]. simpl.
+          exists s. unfold apply_subst.
+          solve_model HR.
+          apply functional_extensionality. intros.
+          specialize (HMod x). simpl in HMod.
+          unfold subst_fresh, stack_subst.
+          destruct (in_dec Rel.dec_eq x xs) as [|HNotIn]; [reflexivity|].
+          apply HMod; assumption.
+        - simpl in HSem. destruct HSem. 
+        - inversion H1; subst.
+          eapply IHframe_trace; try eassumption.
+          solve_model HR.
+        - inversion H1; subst.
+          eapply IHframe_trace; try eassumption.
+          solve_model HR.
+        - inversion H1; subst.
+          eapply IHframe_trace; try eassumption.
+          solve_model HR.
+        - inversion H1; subst.
+          eapply IHframe_trace; try eassumption.
+          solve_model HR.
+      + unfold stptr, protocol in *.
+        simpl in HSem.
+        opt_destruct; [|destruct HSem].
+		destruct s1; destruct HSem. pose proof HPRFrame.
+        simpl in HPRFrame. specialize (HPRFrame x). opt_destruct.
+        destruct HPRFrame as [[H3 H4] | [H3 H4]].
+        rewrite Maps.MF.find_mapsto_iff in H3.
+        unfold stptr in *.
+        rewrite H3 in Heqo. inversion Heqo; subst.
+        simpl. unfold stptr. rewrite <- Heqo0. 
+        split. solve_model H. exists frame. assumption.
+        eapply IHframe_trace; try eassumption.
+        Require Import Charge.SepAlg.SepAlgMap.
+        apply sa_mul_add. assumption. assumption.
+        solve_model HR.
+        rewrite Maps.MF.in_find_iff in H4. contradict H4. intros HNone.
+        unfold stptr in *. rewrite HNone in Heqo. congruence.
+        destruct HPRFrame as [H9 _]. contradict H9.
+        rewrite Maps.MF.in_find_iff. intros HNone. unfold stptr in *. rewrite HNone in Heqo. 
+        congruence.
+      + unfold stptr, protocol in *.
+        simpl in HSem.
+        opt_destruct; [|destruct HSem].
+        destruct s0; try destruct HSem.
+        assert (MapInterface.find c STs = Some (st_recv v s0 s1)) by admit.
+        simpl. unfold stptr, protocol in *. rewrite H0.
+        intros; eapply H; try eassumption; [intros; eapply HMod; eassumption| | eapply HSem; apply H1| solve_model HR].
+		apply sa_mul_add; try assumption.
+		specialize (HPRFrame c). 
+		opt_destruct.
+		destruct HPRFrame as [HPRFrame | [H2 H3]]; [tauto|].
+		contradict H3. rewrite Maps.MF.in_find_iff. intros HNone. rewrite HNone in Heqo. congruence.
+		tauto.
+      + admit.
+   Qed.
+      
+(*    
+    Lemma conj_rule G P1 P2 Q1 Q2 c 
+      (H1 : G |-- {{P1}} c {{Q1}})
+      (H2 : G |-- {{P2}} c {{Q2}}) :
+      G |-- {{P1 //\\ P2}} c {{Q1 //\\ Q2}}.
+    Proof.
+      intros n P HPP HG.
+      simpl. intros m k s h cl pr HPP' Hm Hk [HP1 HP2]. split.
+      + eapply H1; eauto.
+      + intros tr h' s' cl' Hsem.
+        specialize (H1 _ _ HPP); specialize (H1 _ _ _ _ _ cl _ HPP' Hm Hk HP1); destruct H1 as [_ H1]; specialize (H1 _ _ _ _ Hsem).
+        specialize (H2 _ _ HPP); specialize (H2 _ _ _ _ _ cl _ HPP' Hm Hk HP2); destruct H2 as [_ H2]; specialize (H2 _ _ _ _ Hsem).
+        eapply Comp_split; eassumption.
+    Qed.
+*)
+  End StructuralRules.
+
+  Section PrimitivesRules.
+
+    Lemma skip_rule P : |-- {{P}}skip_cmd {{P}}.
+    Proof.
+      intros n Pr HPP Pr' m s h cl pr _ Hmn HP tr HSem.
+      inversion HSem; subst; simpl.
+      apply HP.
+    Qed.
+
+      Lemma trace_append_cmd_Comp Pr Pr' m n P Q tr tr' pr c
+          (HPr : Program.Prog_wf_sub Pr Pr') (Hmn : m <= n) (H : Comp Pr' m pr tr P) 
+          (HTriple : ({{P}} c {{Q}}) Pr n) (Htrace : trace_append_cmd Pr' c tr tr') :
+          Comp Pr' m pr tr' Q.
+      Proof.
+      generalize dependent tr'; generalize dependent pr; generalize dependent m; induction tr; intros.
+      + inversion Htrace.
+      + simpl in H. destruct H.
+      + inversion Htrace; subst.
+        simpl in H. 
+        opt_destruct; [|inversion H].
+        destruct s0; destruct H.
+        simpl. rewrite <- Heqo.
+        split; [assumption|].
+        apply IHtr; try omega; assumption.
+      + inversion Htrace; subst.
+        simpl in H0.
+        opt_destruct; [|inversion H0].
+        destruct s0; try destruct H0.
+        simpl; rewrite <- Heqo. intros.
+        eapply H; try omega. apply H0. eassumption. apply X.
+      + inversion Htrace.
+      + inversion Htrace; subst.
+        * clear IHtr. simpl in H.
+          assert (P s pr Pr' (m - 1) h) by solve_model H.
+		  assert (m - 1 <= n) by omega.
+          specialize (HTriple _ (m - 1) s h t pr HPr H1 H0 _ H5).
+		  simpl; destruct tr0; simpl in *; try congruence. destruct HTriple.
+        * assert (m - 1 <= n) by omega.
+          specialize (IHtr _ H0).
+          destruct tr; simpl in *; inversion X; subst. 
+          - simpl in *. destruct H.
+		  - apply IHtr; assumption. 
+          - apply IHtr; assumption.
+          - apply IHtr; assumption.
+		  - apply IHtr; assumption.       
+      Qed.
+
+    Lemma seq_rule c1 c2 P Q R :
+      ({{P}}c1{{Q}} //\\ {{Q}}c2{{R}}) |-- {{P}}seq_cmd c1 c2{{R}}.
+    Proof.
+      intros Pr n [Hc1 Hc2] Pr' m s h cl pr HPP' Hmn HP tr Hcmd.
+      inversion Hcmd; subst. clear Hcmd.
+      specialize (Hc1 _ _ s h cl pr HPP' Hmn HP tr0 H).
+      clear HP H.
+      eapply trace_append_cmd_Comp; eassumption.
+    Qed.
+
+    Lemma nondet_rule c1 c2 P Q:
+      ({{P}}c1{{Q}} //\\ {{P}}c2{{Q}}) |-- {{P}}nondet_cmd c1 c2{{Q}}.
+    Proof.
+      intros Pr n [Hc1 Hc2] Pr' m s h cl pr HPP' Hmn HP tr Hcmd. inversion Hcmd; subst.
+      + specialize (Hc1 _ _ s h cl pr HPP' Hmn HP _ H). apply Hc1.
+      + specialize (Hc2 _ _ s h cl pr HPP' Hmn HP _ H). apply Hc2.
+    Qed.
+
+    Lemma kleene_rule c P:
+      {{P}}c{{P}} |-- {{P}} kleene_cmd c {{P}}.
+    Proof. 
+      intros Pr n Hc Pr' m k s h cl pr HPP' Hmn tr HSem. 
+      generalize dependent pr; generalize dependent m.
+      induction HSem; simpl; intros.
+      - apply Hmn.
+      - eapply trace_append_cmd_Comp; try eassumption.
+        simpl in Hc. eapply Hc; eassumption.
+    Qed.
+
+    Lemma assume_rule P (t : vlogic) :
+      |-- {{P}} assume_cmd t {{t /\\ P}}.
+    Proof.
+      intros Pr n Hc Pr' m s h cl pr HPP' Hmn Hp tr Hcmd.
+      inversion Hcmd; subst.
+      simpl. split. assumption. solve_model Hp.
+    Qed.
+
+    Lemma assert_rule (P : psasn) (p : vlogic) (HPe : P |-- embed p) :
+      |-- {{P}} assert_cmd p {{P}}.
+    Proof.
+      intros n Pr Hc Pr' m s h cl pr HPP' Hmn Hp tr Hcmd. 
+	  specialize (HPe _ _ _ _ _ Hp).
+	  inversion Hcmd; subst. simpl. apply Hp.
+	  simpl in *. apply HNP. apply HPe.
+    Qed.
+    
+  End PrimitivesRules.
+
+  Lemma exists_into_precond {A} (P: A -> psasn) c q :
+    (Forall x, {{P x}} c {{q}}) -|- {{Exists x, P x}} c {{q}}.
+  Proof.
+  	split.
+  	+ intros Pr n Hc Pr' m s h cl pr HPP' Hmn [x Hp] tr HSem. specialize (Hc x).
+  	  simpl in *. eapply Hc; eassumption.
+  	+ intros Pr n Hc x Pr' m k s h cl HPP' Hmn  Hxp tr HSem.
+  	  simpl in Hc; eapply Hc; try eassumption. exists x; apply Hxp.
+  Qed.
+
+  (* Holds only in one direction unless annotations on assertion logic, which is ugly - well, it's happened. - F.
+     This is the important direction, though *)
+  Lemma I_precond (SP : spec) (P Q : psasn) c:
+    (SP -->> {{ P }} c {{ Q }}) -|- {{ SP /\\  P }} c {{ Q }}.
+  Proof.
+  	split.
+  	+ intros n Pr Hc Pr' m k s h cl HPP' Hmn [HSP HP] tr HSem.
+  	  specialize (Hc Pr' HPP' m Hmn HSP).
+  	  simpl in Hc. eapply Hc; reflexivity || eassumption.
+  	+ intros Pr n Hc Pr' HPP' m Hnm HSP Pr'' l s h pr cl HPP'' Hlm HP tr HSem.
+  	  simpl in Hc; eapply Hc.
+  	  * transitivity Pr'; assumption.
+  	  * omega.
+  	  * simpl. split. 
+        assert ((SP Pr'') l). solve_model HSP. intros a b. simpl. intuition.
+        apply H. apply HP. 
+      * eassumption.
+  Qed.
+
+End Rules.
